feat: smc_rec_destroy

container/coq/pointer/Layer10/Layer.v
@@ -3,6 +3,7 @@ Require Import CommonDeps.
 Require Import DataTypes.
 Require Import GlobalDefs.
 Require Import Layer1.Spec.
+Require Import Layer10.Spec.
 Require Import Layer2.Spec.
 Require Import Layer3.Spec.
 Require Import Layer4.Spec.
@@ -14,33 +15,33 @@ Require Import Layer8.Spec.
 Local Open Scope string_scope.
 Local Open Scope Z_scope.
 
-Parameter Layer8_init: RData.
+Parameter Layer10_init: RData.
 
-Section Layer8_Layer.
+Section Layer10_Layer.
 
   Context `{int_ptr: IntPtrCast}.
 
-  Definition Layer8_get_reg (reg: regset) (st: RData) : option Z := None.
+  Definition Layer10_get_reg (reg: regset) (st: RData) : option Z := None.
 
-  Definition Layer8_set_reg (reg: regset) (val: Z) (st: RData) : option RData := None.
+  Definition Layer10_set_reg (reg: regset) (val: Z) (st: RData) : option RData := None.
 
-  Definition Layer8_get_flag (f: flag) (st: RData) : bool := false.
+  Definition Layer10_get_flag (f: flag) (st: RData) : bool := false.
 
-  Definition Layer8_set_flag (f: flag) (val: bool) (st: RData) : option RData := None.
+  Definition Layer10_set_flag (f: flag) (val: bool) (st: RData) : option RData := None.
 
-  Definition Layer8_layer :=
+  Definition Layer10_layer :=
     {|
       State := RData;
-      Init := Layer8_init;
+      Init := Layer10_init;
       Load := load_RData;
       Store := store_RData;
       NewFrame := new_frame;
       Alloca := alloc_stack;
       Free := free_stack;
-      GetReg :=Layer8_get_reg;
-      SetReg := Layer8_set_reg;
-      GetFlag := Layer8_get_flag;
-      SetFlag := Layer8_set_flag;
+      GetReg :=Layer10_get_reg;
+      SetReg := Layer10_set_reg;
+      GetFlag := Layer10_get_flag;
+      SetFlag := Layer10_set_flag;
       Ptr2Int := ptr_to_int;
       Int2Ptr := int_to_ptr;
       PtrEqb := ptr_eqb;
@@ -62,7 +63,7 @@ Section Layer8_Layer.
           :: ("atomic_granule_get", prim atomic_granule_get_spec)
           :: ("atomic_granule_put", prim atomic_granule_put_spec)
           :: ("atomic_load_add_release_64", prim atomic_load_add_release_64_spec)
-          :: ("data_create_internal", prim data_create_internal_spec)
+          :: ("data_create_s1_el1", prim data_create_s1_el1_spec)
           :: ("esr_is_write", prim esr_is_write_spec)
           :: ("esr_srt", prim esr_srt_spec)
           :: ("esr_sysreg_rt", prim esr_sysreg_rt_spec)
@@ -70,42 +71,38 @@ Section Layer8_Layer.
           :: ("find_lock_granule", prim find_lock_granule_spec)
           :: ("find_lock_two_granules", prim find_lock_two_granules_spec)
           :: ("g_refcount", prim g_refcount_spec)
+          :: ("gic_restore_state", prim gic_restore_state_spec)
           :: ("granule_addr", prim granule_addr_spec)
           :: ("granule_lock", prim granule_lock_spec)
           :: ("granule_map", prim granule_map_spec)
+          :: ("granule_memzero", prim granule_memzero_spec)
           :: ("granule_memzero_mapped", prim granule_memzero_mapped_spec)
           :: ("granule_pa_to_va", prim granule_pa_to_va_spec)
+          :: ("granule_refcount_read_acquire", prim granule_refcount_read_acquire_spec)
           :: ("granule_set_state", prim granule_set_state_spec)
-          :: ("granule_try_lock", prim granule_try_lock_spec)
           :: ("granule_unlock", prim granule_unlock_spec)
           :: ("granule_unlock_transition", prim granule_unlock_transition_spec)
           :: ("invalidate_block", prim invalidate_block_spec)
           :: ("invalidate_pages_in_block", prim invalidate_pages_in_block_spec)
-          :: ("is_addr_in_par", prim is_addr_in_par_spec)
           :: ("llvm_memcpy_p0i8_p0i8_i64", prim llvm_memcpy_p0i8_p0i8_i64_spec)
           :: ("make_return_code", prim make_return_code_spec)
-          :: ("masked_assign", prim masked_assign_spec)
+          :: ("map_unmap_ns_s1", prim map_unmap_ns_s1_spec)
           :: ("max_pa_size", prim max_pa_size_spec)
           :: ("memcpy_ns_write", prim memcpy_ns_write_spec)
           :: ("memset", prim memset_spec)
           :: ("ns_buffer_read", prim ns_buffer_read_spec)
-          :: ("ns_buffer_read_byte", prim ns_buffer_read_byte_spec)
           :: ("ns_buffer_unmap", prim ns_buffer_unmap_spec)
-          :: ("ns_buffer_write_byte", prim ns_buffer_write_byte_spec)
           :: ("pack_return_code", prim pack_return_code_spec)
           :: ("pack_struct_return_code", prim pack_struct_return_code_spec)
           :: ("pico_rec_enter", prim pico_rec_enter_spec)
           :: ("ranges_intersect", prim ranges_intersect_spec)
           :: ("realm_ipa_bits", prim realm_ipa_bits_spec)
-          :: ("realm_ipa_size", prim realm_ipa_size_spec)
           :: ("realm_rtt_starting_level", prim realm_rtt_starting_level_spec)
           :: ("rec_run_loop", prim rec_run_loop_spec)
           :: ("region_is_contained", prim region_is_contained_spec)
-          :: ("rtt_create_internal", prim rtt_create_internal_spec)
+          :: ("rmm_feature_register_0_value", prim rmm_feature_register_0_value_spec)
+          :: ("rtt_create_s1_el1", prim rtt_create_s1_el1_spec)
           :: ("rtt_walk_lock_unlock", prim rtt_walk_lock_unlock_spec)
-          :: ("s1addr_is_level_aligned", prim s1addr_is_level_aligned_spec)
-          :: ("s1tte_is_valid", prim s1tte_is_valid_spec)
-          :: ("s1tte_pa", prim s1tte_pa_spec)
           :: ("s2tt_init_unassigned", prim s2tt_init_unassigned_spec)
           :: ("s2tte_create_assigned", prim s2tte_create_assigned_spec)
           :: ("s2tte_create_table", prim s2tte_create_table_spec)
@@ -118,21 +115,17 @@ Section Layer8_Layer.
           :: ("s2tte_map_size", prim s2tte_map_size_spec)
           :: ("s2tte_pa", prim s2tte_pa_spec)
           :: ("set_rd_state", prim set_rd_state_spec)
-          :: ("set_tte_ns", prim set_tte_ns_spec)
           :: ("spinlock_acquire", prim spinlock_acquire_spec)
           :: ("spinlock_release", prim spinlock_release_spec)
-          :: ("stage1_tlbi_all", prim stage1_tlbi_all_spec)
           :: ("table_is_destroyed_block", prim table_is_destroyed_block_spec)
           :: ("table_is_unassigned_block", prim table_is_unassigned_block_spec)
           :: ("table_maps_assigned_block", prim table_maps_assigned_block_spec)
           :: ("table_maps_valid_block", prim table_maps_valid_block_spec)
           :: ("table_maps_valid_ns_block", prim table_maps_valid_ns_block_spec)
           :: ("validate_gic_state", prim validate_gic_state_spec)
+          :: ("validate_map_addr", prim validate_map_addr_spec)
           :: ("validate_ns_struct", prim validate_ns_struct_spec)
-          :: ("write_ap0r", prim write_ap0r_spec)
-          :: ("write_ap1r", prim write_ap1r_spec)
-          :: ("write_lr", prim write_lr_spec)
           :: nil
     |}.
 
-End Layer8_Layer.
+End Layer10_Layer.
