container/coq/pointer/.CachedSpec/Layer11Spec.v
@@ -1,0 +1,3 @@
+Definition status_ptr_spec (v_0: Z) (st: RData) : (option (Ptr * RData)) :=
+  (Some ((int_to_ptr (0 - (v_0))), st)).
+
