container/coq/pointer/.CachedSpec/Layer4Spec.v
@@ -6,27 +6,6 @@ Definition cpuid_spec (st: RData) : (option (Z * RData)) :=
 Definition find_granule_spec_abs (v_0: abs_PA_t) (st: RData) : (option (Ptr * RData)) :=
   (Some ((mkPtr "granules" (v_0.(meta_granule_offset))), st)).
 
-Definition __find_next_level_idx_spec (v_0: Ptr) (v_1: Z) (st: RData) : (option (Ptr * RData)) :=
-  if (((abs_tte_read (mkPtr "granule_data" ((v_0.(poffset)) + ((8 * (v_1))))) st).(meta_desc_type)) =? (3))
-  then (Some ((mkPtr "granules" (((abs_tte_read (mkPtr "granule_data" ((v_0.(poffset)) + ((8 * (v_1))))) st).(meta_PA)).(meta_granule_offset))), st))
-  else (Some ((mkPtr "null" 0), st)).
-
-Definition s2_addr_to_idx_spec (v_0: Z) (v_1: Z) (st: RData) : (option (Z * RData)) :=
-  (Some ((s2_addr_to_idx_para v_0 v_1), st)).
-
 Definition find_granule_spec (v_0: Z) (st: Z) : (option (Ptr * RData)) :=
   None.
-
-Definition granule_lock_spec (v_0: Ptr) (v_1: Z) (st: RData) : (option RData) :=
-  when st_1 == ((spinlock_acquire_spec (mkPtr (v_0.(pbase)) (v_0.(poffset))) st));
-  if (((((((st_1.(share)).(globals)).(g_granules)) @ ((v_0.(poffset)) / (16))).(e_state_s_granule)) - (v_1)) =? (0))
-  then (Some st_1)
-  else (
-    when st_2 == ((spinlock_release_spec (mkPtr (v_0.(pbase)) (v_0.(poffset))) st_1));
-    (Some st_2)).
-
-Definition s2tte_create_ripas_spec (v_0: Z) (st: RData) : (option (Z * RData)) :=
-  if (v_0 =? (0))
-  then (Some (0, st))
-  else (Some (64, st)).
 
