container/coq/pointer/.CachedSpec/Layer5Spec.v
@@ -54,29 +54,15 @@ Definition atomic_add_64 (loc: Ptr) (val: Z) (st: RData) : (option RData) :=
   when st_2 == ((store_RData_granules 64 loc (v + (val)) st_1));
   (Some st_2).
 
-Definition s2tte_is_table_spec (v_0: Z) (v_1: Z) (st: RData) : (option (bool * RData)) :=
-  (Some (((v_1 <? (3)) && (((v_0 & (3)) =? (3)))), st)).
+Definition __granule_put_spec (v_0: Ptr) (st: RData) : (option RData) :=
+  rely (((((v_0.(pbase)) = ("granules")) /\ ((((v_0.(poffset)) mod (16)) = (0)))) /\ (((v_0.(poffset)) >= (0)))));
+  rely (((((v_0.(pbase)) = ("granules")) /\ ((((v_0.(poffset)) mod (16)) = (0)))) /\ (((v_0.(poffset)) >= (0)))));
+  when st_1 == ((atomic_add_64 (ptr_offset v_0 8) (- 1) st));
+  (Some st_1).
 
 Definition granule_unlock_spec (v_0: Ptr) (st: RData) : (option RData) :=
   when st_0 == ((spinlock_release_spec (mkPtr (v_0.(pbase)) (v_0.(poffset))) st));
   (Some st_0).
-
-Definition s2_sl_addr_to_idx_spec (v_0: Z) (v_1: Z) (v_2: Z) (st: RData) : (option (Z * RData)) :=
-  (Some ((((Z.lxor ((- 1) << ((v_2 & (4294967295)))) (- 1)) & (v_0)) >> ((39 + (((- 9) * (v_1)))))), st)).
-
-Definition __find_lock_next_level_spec (v_0: Ptr) (v_1: Z) (v_2: Z) (st: RData) : (option (Ptr * RData)) :=
-  if (((abs_tte_read (mkPtr "granule_data" ((v_0.(poffset)) + ((8 * ((s2_addr_to_idx_para v_1 v_2)))))) st).(meta_desc_type)) =? (3))
-  then (
-    when st_4 == (
-        (granule_lock_spec
-          (mkPtr "granules" (((abs_tte_read (mkPtr "granule_data" ((v_0.(poffset)) + ((8 * ((s2_addr_to_idx_para v_1 v_2)))))) st).(meta_PA)).(meta_granule_offset)))
-          5
-          st));
-    (Some (
-      (mkPtr "granules" (((abs_tte_read (mkPtr "granule_data" ((v_0.(poffset)) + ((8 * ((s2_addr_to_idx_para v_1 v_2)))))) st).(meta_PA)).(meta_granule_offset)))  ,
-      st_4
-    )))
-  else (Some ((mkPtr "null" 0), st)).
 
 Definition pack_struct_return_code_spec (v_0: Z) (st: RData) : (option (Z * RData)) :=
   (Some ((pack_struct_return_code_para v_0), st)).
@@ -96,9 +82,4 @@ Definition atomic_granule_put_spec (v_0: Ptr) (st: RData) : (option RData) :=
 
 Definition find_lock_granule_spec (v_0: Z) (v_1: Z) (st: RData) : (option (Ptr * RData)) :=
   None.
-
-Definition s2tte_create_unassigned_spec (v_0: Z) (st: RData) : (option (Z * RData)) :=
-  if (v_0 =? (0))
-  then (Some (0, st))
-  else (Some (64, st)).
 
