container/coq/pointer/.CachedSpec/Layer8Spec.v
@@ -209,7 +209,3 @@ Definition data_create_s1_el1_spec_abs (v_0_pte: abs_PTE_t) (v_1_pa: abs_PA_t) (
       when st_2 == ((spinlock_release_spec (mkPtr "granules" ((v_0_pte.(meta_PA)).(meta_granule_offset))) st_1));
       (Some ((pack_struct_return_code_para (make_return_code_para 3)), st_2)))).
 
-Definition granule_memzero_spec (v_0: Ptr) (v_1: Z) (st: RData) : (option RData) :=
-  when v_4, st_1 == ((memset_spec (mkPtr "granule_data" (v_0.(poffset))) 0 4096 st));
-  (Some st_1).
-
