container/coq/pointer/Layer11/status_ptr/CodeProof.v
@@ -1,27 +1,26 @@
-Require Import Bottom.Spec.
 Require Import Code.
 Require Import CommonDeps.
 Require Import DataTypes.
 Require Import GlobalDefs.
-Require Import Layer7.Layer.
-Require Import Layer8.granule_memzero_mapped.LowSpec.
+Require Import Layer10.Layer.
+Require Import Layer11.status_ptr.LowSpec.
 Require Import Zwf.
 
 Local Open Scope string_scope.
 Local Open Scope Z_scope.
 Local Opaque Z.add Z.mul Z.div Z.sub Z.land Z.lor Z.lxor Z.shiftl Z.shiftr Z.quot Z.rem Z.testbit Z.setbit Z.clearbit xorb List.nth.
 
-Section Layer8_granule_memzero_mapped_CodeProof.
+Section Layer11_status_ptr_CodeProof.
 
   Context `{int_ptr: IntPtrCast}.
 
-  Local Opaque memset_spec.
-    Lemma f_granule_memzero_mapped_correct:
-      forall v_0 st st'
-             (Hspec: granule_memzero_mapped_spec_low v_0 st = Some st'),
-        exec_func Layer7_layer code "granule_memzero_mapped"
-                  [VPtr v_0]
-                  st st' None.
+  Local Opaque int_to_ptr.
+    Lemma f_status_ptr_correct:
+      forall v_0 st st' res
+             (Hspec: status_ptr_spec_low v_0 st = Some (res, st')),
+        exec_func Layer10_layer code "status_ptr"
+                  [VInt v_0]
+                  st st' (Some (VPtr res)).
     Proof.
         intros; simpl_func Hspec; simpl in *;
           unshelve (eapply exec_func_call);
@@ -41,5 +40,5 @@ Section Layer8_granule_memzero_mapped_CodeProof.
           end).
     Qed.
 
-End Layer8_granule_memzero_mapped_CodeProof.
+End Layer11_status_ptr_CodeProof.
 
