container/coq/pointer/Layer4/Spec.v
@@ -1,8 +1,6 @@
 Require Import CommonDeps.
 Require Import DataTypes.
 Require Import GlobalDefs.
-Require Import Layer2.Spec.
-Require Import Layer3.Spec.
 
 Local Open Scope string_scope.
 Local Open Scope Z_scope.
@@ -19,36 +17,11 @@ Section Layer4_Spec.
   Definition find_granule_spec_abs (v_0: abs_PA_t) (st: RData) : (option (Ptr * RData)) :=
     (Some ((mkPtr "granules" (v_0.(meta_granule_offset))), st)).
 
-  Definition __find_next_level_idx_spec (v_0: Ptr) (v_1: Z) (st: RData) : (option (Ptr * RData)) :=
-    if (((abs_tte_read (mkPtr "granule_data" ((v_0.(poffset)) + ((8 * (v_1))))) st).(meta_desc_type)) =? (3))
-    then (Some ((mkPtr "granules" (((abs_tte_read (mkPtr "granule_data" ((v_0.(poffset)) + ((8 * (v_1))))) st).(meta_PA)).(meta_granule_offset))), st))
-    else (Some ((mkPtr "null" 0), st)).
-
-  Definition s2_addr_to_idx_spec (v_0: Z) (v_1: Z) (st: RData) : (option (Z * RData)) :=
-    (Some ((s2_addr_to_idx_para v_0 v_1), st)).
-
   Definition find_granule_spec (v_0: Z) (st: Z) : (option (Ptr * RData)) :=
     None.
-
-  Definition granule_lock_spec (v_0: Ptr) (v_1: Z) (st: RData) : (option RData) :=
-    when st_1 == ((spinlock_acquire_spec (mkPtr (v_0.(pbase)) (v_0.(poffset))) st));
-    if (((((((st_1.(share)).(globals)).(g_granules)) @ ((v_0.(poffset)) / (16))).(e_state_s_granule)) - (v_1)) =? (0))
-    then (Some st_1)
-    else (
-      when st_2 == ((spinlock_release_spec (mkPtr (v_0.(pbase)) (v_0.(poffset))) st_1));
-      (Some st_2)).
-
-  Definition s2tte_create_ripas_spec (v_0: Z) (st: RData) : (option (Z * RData)) :=
-    if (v_0 =? (0))
-    then (Some (0, st))
-    else (Some (64, st)).
 
 End Layer4_Spec.
 
 #[global] Hint Unfold cpuid_spec: spec.
 #[global] Hint Unfold find_granule_spec_abs: spec.
-#[global] Hint Unfold __find_next_level_idx_spec: spec.
-#[global] Hint Unfold s2_addr_to_idx_spec: spec.
 #[global] Hint Unfold find_granule_spec: spec.
-Opaque granule_lock_spec.
-#[global] Hint Unfold s2tte_create_ripas_spec: spec.
