container/coq/pointer/Layer5/Spec.v
@@ -1,9 +1,7 @@
 Require Import CommonDeps.
 Require Import DataTypes.
 Require Import GlobalDefs.
-Require Import Layer2.Spec.
 Require Import Layer3.Spec.
-Require Import Layer4.Spec.
 Require Import Layer6.Spec.
 
 Local Open Scope string_scope.
@@ -69,29 +67,15 @@ Section Layer5_Spec.
     when st_2 == ((store_RData_granules 64 loc (v + (val)) st_1));
     (Some st_2).
 
-  Definition s2tte_is_table_spec (v_0: Z) (v_1: Z) (st: RData) : (option (bool * RData)) :=
-    (Some (((v_1 <? (3)) && (((v_0 & (3)) =? (3)))), st)).
+  Definition __granule_put_spec (v_0: Ptr) (st: RData) : (option RData) :=
+    rely (((((v_0.(pbase)) = ("granules")) /\ ((((v_0.(poffset)) mod (16)) = (0)))) /\ (((v_0.(poffset)) >= (0)))));
+    rely (((((v_0.(pbase)) = ("granules")) /\ ((((v_0.(poffset)) mod (16)) = (0)))) /\ (((v_0.(poffset)) >= (0)))));
+    when st_1 == ((atomic_add_64 (ptr_offset v_0 8) (- 1) st));
+    (Some st_1).
 
   Definition granule_unlock_spec (v_0: Ptr) (st: RData) : (option RData) :=
     when st_0 == ((spinlock_release_spec (mkPtr (v_0.(pbase)) (v_0.(poffset))) st));
     (Some st_0).
-
-  Definition s2_sl_addr_to_idx_spec (v_0: Z) (v_1: Z) (v_2: Z) (st: RData) : (option (Z * RData)) :=
-    (Some ((((Z.lxor ((- 1) << ((v_2 & (4294967295)))) (- 1)) & (v_0)) >> ((39 + (((- 9) * (v_1)))))), st)).
-
-  Definition __find_lock_next_level_spec (v_0: Ptr) (v_1: Z) (v_2: Z) (st: RData) : (option (Ptr * RData)) :=
-    if (((abs_tte_read (mkPtr "granule_data" ((v_0.(poffset)) + ((8 * ((s2_addr_to_idx_para v_1 v_2)))))) st).(meta_desc_type)) =? (3))
-    then (
-      when st_4 == (
-          (granule_lock_spec
-            (mkPtr "granules" (((abs_tte_read (mkPtr "granule_data" ((v_0.(poffset)) + ((8 * ((s2_addr_to_idx_para v_1 v_2)))))) st).(meta_PA)).(meta_granule_offset)))
-            5
-            st));
-      (Some (
-        (mkPtr "granules" (((abs_tte_read (mkPtr "granule_data" ((v_0.(poffset)) + ((8 * ((s2_addr_to_idx_para v_1 v_2)))))) st).(meta_PA)).(meta_granule_offset)))  ,
-        st_4
-      )))
-    else (Some ((mkPtr "null" 0), st)).
 
   Definition pack_struct_return_code_spec (v_0: Z) (st: RData) : (option (Z * RData)) :=
     (Some ((pack_struct_return_code_para v_0), st)).
@@ -112,11 +96,6 @@ Section Layer5_Spec.
   Definition find_lock_granule_spec (v_0: Z) (v_1: Z) (st: RData) : (option (Ptr * RData)) :=
     None.
 
-  Definition s2tte_create_unassigned_spec (v_0: Z) (st: RData) : (option (Z * RData)) :=
-    if (v_0 =? (0))
-    then (Some (0, st))
-    else (Some (64, st)).
-
 End Layer5_Spec.
 
 #[global] Hint Unfold s2tte_create_unassigned_spec_abs: spec.
@@ -129,12 +108,9 @@ Opaque memcpy_ns_read_spec.
 #[global] Hint Unfold __find_lock_next_level_spec_low_abs: spec.
 #[global] Hint Unfold find_lock_granule_spec_abs: spec.
 #[global] Hint Unfold atomic_add_64: spec.
-#[global] Hint Unfold s2tte_is_table_spec: spec.
+#[global] Hint Unfold __granule_put_spec: spec.
 Opaque granule_unlock_spec.
-#[global] Hint Unfold s2_sl_addr_to_idx_spec: spec.
-#[global] Hint Unfold __find_lock_next_level_spec: spec.
 #[global] Hint Unfold pack_struct_return_code_spec: spec.
 #[global] Hint Unfold make_return_code_spec: spec.
 #[global] Hint Unfold atomic_granule_put_spec: spec.
 #[global] Hint Unfold find_lock_granule_spec: spec.
-#[global] Hint Unfold s2tte_create_unassigned_spec: spec.
