container/coq/pointer/Layer6/Spec.v
@@ -1,9 +1,7 @@
 Require Import CommonDeps.
 Require Import DataTypes.
 Require Import GlobalDefs.
-Require Import Layer2.Spec.
 Require Import Layer3.Spec.
-Require Import Layer4.Spec.
 Require Import Layer5.Spec.
 
 Local Open Scope string_scope.
@@ -122,14 +120,6 @@ Section Layer6_Spec.
           when i, s == ((s2_addr_to_idx_spec v_4 2 st_6));
           (Some ((mkabs_ret_rtt 3 ret_3 i), s))))).
 
-  Definition s2tte_pa_spec (v_0: Z) (v_1: Z) (st: RData) : (option (Z * RData)) :=
-    if ((v_1 <? (3)) && (((v_0 & (3)) =? (3))))
-    then (Some (((v_0 & (281474976710655)) & (((- 1) << (12)))), st))
-    else (Some (((v_0 & (281474976710655)) & (((- 1) << (((39 + (((- 9) * (v_1)))) & (4294967295)))))), st)).
-
-  Definition rtt_walk_lock_unlock_spec (v_0: Ptr) (v_1: Ptr) (v_2: Z) (v_3: Z) (v_4: Z) (v_5: Z) (st: RData) : (option RData) :=
-    None.
-
   Definition granule_set_state_spec (v_0: Ptr) (v_1: Z) (st: RData) : (option RData) :=
     rely ((((v_0.(poffset)) mod (16)) = (0)));
     (Some (st.[share].[globals].[g_granules] :<
@@ -139,23 +129,6 @@ Section Layer6_Spec.
 
   Definition pack_return_code_spec (v_0: Z) (v_1: Z) (st: RData) : (option (Z * RData)) :=
     (Some ((pack_struct_return_code_para (make_return_code_para v_0)), st)).
-
-  Definition g_refcount_spec (v_0: Ptr) (st: RData) : (option (Z * RData)) :=
-    rely (((((v_0.(pbase)) = ("granules")) /\ ((((v_0.(poffset)) mod (16)) = (0)))) /\ (((v_0.(poffset)) >= (0)))));
-    when v_3, st_0 == ((load_RData 8 (mkPtr (v_0.(pbase)) ((v_0.(poffset)) + (8))) st));
-    (Some ((v_3 & (4095)), st_0)).
-
-  Definition __granule_put_spec (v_0: Ptr) (st: RData) : (option RData) :=
-    rely (((((v_0.(pbase)) = ("granules")) /\ ((((v_0.(poffset)) mod (16)) = (0)))) /\ (((v_0.(poffset)) >= (0)))));
-    (Some (st.[share].[globals].[g_granules] :<
-      ((((st.(share)).(globals)).(g_granules)) #
-        ((v_0.(poffset)) / (16)) ==
-        (((((st.(share)).(globals)).(g_granules)) @ ((v_0.(poffset)) / (16))).[e_ref] :<
-          ((((((st.(share)).(globals)).(g_granules)) @ ((v_0.(poffset)) / (16))).(e_ref)).[e_u_anon_3_0] :<
-            (((((((st.(share)).(globals)).(g_granules)) @ ((v_0.(poffset)) / (16))).(e_ref)).(e_u_anon_3_0)) + ((- 1)))))))).
-
-  Definition stage1_tlbi_all_spec (st: RData) : (option RData) :=
-    (Some st).
 
 End Layer6_Spec.
 
@@ -175,10 +148,5 @@ Opaque __tte_write_spec.
 #[global] Hint Unfold s2tt_init_unassigned_loop759_rank: spec.
 #[global] Hint Unfold s2tt_init_unassigned_loop759_0_rank: spec.
 Opaque rtt_walk_lock_unlock_spec_abs.
-#[global] Hint Unfold s2tte_pa_spec: spec.
-Opaque rtt_walk_lock_unlock_spec.
 #[global] Hint Unfold granule_set_state_spec: spec.
 #[global] Hint Unfold pack_return_code_spec: spec.
-#[global] Hint Unfold g_refcount_spec: spec.
-#[global] Hint Unfold __granule_put_spec: spec.
-#[global] Hint Unfold stage1_tlbi_all_spec: spec.
